pulse/share/steel/examples/pulse/lib/Pulse.Lib.Array.fst
@@ -17,13 +17,13 @@ let coerce (#t:Type) (l:US.t) (s:Ghost.erased (elseq t l)) : Ghost.erased (Seq.s
 fn compare_ (#t:eqtype) (l:US.t) (a1 a2:larray t (US.v l))
            (#p1 #p2:perm) (#s1 #s2:Ghost.erased (elseq t l))
   requires (
-    A.pts_to a1 p1 s1 **
-    A.pts_to a2 p2 s2
+    A.pts_to a1 #p1 s1 **
+    A.pts_to a2 #p2 s2
   )
   returns res:bool
   ensures (
-    A.pts_to a1 p1 s1 **
-    A.pts_to a2 p2 s2 **
+    A.pts_to a1 #p1 s1 **
+    A.pts_to a2 #p2 s2 **
     (pure (res <==> Seq.equal s1 s2))
   )
 {
@@ -35,9 +35,9 @@ fn compare_ (#t:eqtype) (l:US.t) (a1 a2:larray t (US.v l))
       (v1 = v2) } 
     else { false } )
   invariant b. exists (vi:US.t). ( 
-    R.pts_to i full_perm vi **
-    A.pts_to a1 p1 s1 **
-    A.pts_to a2 p2 s2 **
+    R.pts_to i vi **
+    A.pts_to a1 #p1 s1 **
+    A.pts_to a2 #p2 s2 **
     pure (
       vi <= l /\
       (b == (vi < l && Seq.index s1 (US.v vi) = Seq.index s2 (US.v vi))) /\
@@ -65,20 +65,20 @@ let lemma_seq_equal (#t:eqtype) (l:US.t) (s1 s2: elseq t l)
 fn memcpy_ (#t:eqtype) (l:US.t) (src dst:larray t (US.v l))
           (#p:perm) (#src0 #dst0:Ghost.erased (elseq t l))
   requires (
-    A.pts_to src p src0 **
-    A.pts_to dst full_perm dst0
+    A.pts_to src #p src0 **
+    A.pts_to dst dst0
   )
   ensures (
-    A.pts_to src p src0 **
-    A.pts_to dst full_perm src0
+    A.pts_to src #p src0 **
+    A.pts_to dst src0
   )
 {
   let mut i = 0sz;
   while (let vi = !i; (vi < l) )
   invariant b. exists (vi:US.t) (s:elseq t l). ( 
-    R.pts_to i full_perm vi **
-    A.pts_to src p src0 **
-    A.pts_to dst full_perm s **
+    R.pts_to i vi **
+    A.pts_to src #p src0 **
+    A.pts_to dst s **
     pure (
       vi <= l /\
       (b == (vi < l)) /\
@@ -88,12 +88,12 @@ fn memcpy_ (#t:eqtype) (l:US.t) (src dst:larray t (US.v l))
   {
     let vi = !i;
     let x = op_Array_Access src vi #p #(coerce l src0);
-    with s. assert (A.pts_to dst full_perm s);
+    with s. assert (A.pts_to dst s);
     op_Array_Assignment dst vi x #(coerce l s);
     i := vi + 1sz;
     ()
   };
-  with s. assert (A.pts_to dst full_perm s);
+  with s. assert (A.pts_to dst s);
   lemma_seq_equal l src0 s;
   ()
 }
@@ -104,17 +104,17 @@ let memcpy = memcpy_
 ```pulse
 fn fill_ (#t:Type0) (l:US.t) (a:(a:array t{ US.v l == A.length a })) (v:t)
                (#s:Ghost.erased (elseq t l))
-  requires (A.pts_to a full_perm s)
+  requires (A.pts_to a s)
   ensures exists (s:Seq.seq t). (
-    A.pts_to a full_perm s **
+    A.pts_to a s **
     pure (s `Seq.equal` Seq.create (US.v l) v)
   )
 {
    let mut i = 0sz;
    while (let vi = !i; (vi < l))
    invariant b. exists (s:Seq.seq t) (vi:US.t). ( 
-      A.pts_to a full_perm s **
-      R.pts_to i full_perm vi **
+      A.pts_to a s **
+      R.pts_to i vi **
       pure ((b == (vi < l)) /\
             vi <= l /\
             Seq.length s == A.length a /\
@@ -134,9 +134,9 @@ let fill = fill_
 ```pulse
 fn zeroize_ (l:US.t) (a:(a:A.array U8.t{ US.v l == A.length a }))
                  (#s:Ghost.erased (elseq U8.t l))
-  requires A.pts_to a full_perm s
+  requires A.pts_to a s
   ensures exists (s:Seq.seq U8.t). (
-    A.pts_to a full_perm s **
+    A.pts_to a s **
     pure (s `Seq.equal` Seq.create (US.v l) 0uy)
   )
 {
