pulse/share/steel/examples/pulse/lib/Pulse.Lib.Reference.fsti
@@ -1,4 +1,5 @@
 module Pulse.Lib.Reference
+open FStar.Tactics
 open Pulse.Lib.Core
 open Steel.FractionalPermission
 open FStar.Ghost
@@ -6,33 +7,33 @@ module U32 = FStar.UInt32
 
 val ref (a:Type u#0) : Type u#0
 
-val pts_to (#a:Type) (r:ref a) (p:perm) (n:a) : vprop
+val pts_to (#a:Type) (r:ref a) (#[exact (`full_perm)]p:perm) (n:a) : vprop
 
 val alloc (#a:Type) (x:a)
-  : stt (ref a) emp (fun r -> pts_to r full_perm x)
+  : stt (ref a) emp (fun r -> pts_to r x)
   
 val ( ! ) (#a:Type) (r:ref a) (#n:erased a) (#p:perm)
   : stt a
-        (pts_to r p n)
-        (fun x -> pts_to r p x ** pure (reveal n == x))
+        (pts_to r #p n)
+        (fun x -> pts_to r #p x ** pure (reveal n == x))
 
 val ( := ) (#a:Type) (r:ref a) (x:a) (#n:erased a)
   : stt unit
-        (pts_to r full_perm n) 
-        (fun _ -> pts_to r full_perm (hide x))
+        (pts_to r n) 
+        (fun _ -> pts_to r (hide x))
 
 val free (#a:Type) (r:ref a) (#n:erased a)
-  : stt unit (pts_to r full_perm n) (fun _ -> emp)
+  : stt unit (pts_to r n) (fun _ -> emp)
 
 val read_atomic (r:ref U32.t) (#n:erased U32.t) (#p:perm)
   : stt_atomic U32.t emp_inames
-    (pts_to r p n)
-    (fun x -> pts_to r p n ** pure (reveal n == x))
+    (pts_to r #p n)
+    (fun x -> pts_to r #p n ** pure (reveal n == x))
 
 val write_atomic (r:ref U32.t) (x:U32.t) (#n:erased U32.t)
   : stt_atomic unit emp_inames
-        (pts_to r full_perm n) 
-        (fun _ -> pts_to r full_perm (hide x))
+        (pts_to r n) 
+        (fun _ -> pts_to r (hide x))
 
 val with_local
   (#a:Type0)
@@ -40,6 +41,6 @@ val with_local
   (#pre:vprop)
   (#ret_t:Type)
   (#post:ret_t -> vprop)
-  (body:(r:ref a) -> stt ret_t (pre ** pts_to r full_perm init)
-                               (fun v -> post v ** exists_ (pts_to r full_perm)))
+  (body:(r:ref a) -> stt ret_t (pre ** pts_to r init)
+                              (fun v -> post v ** exists_ (pts_to r)))
   : stt ret_t pre post
